Trying to improve the closLang semantic relation
We want flexibility for the compiler to change the number of clock steps
required, but we have to be careful that relation implies divergence
preservation. The relation here is trying to use an unbounded, monotone
function, but the quantification structure doesn't work out. I'll have
to try something more complex.

new-backend/clos_relationScript.sml
@@ -71,76 +71,104 @@ val (val_rel_rules, val_rel_ind, val_rel_cases) = Hol_reln `
 *)
 
 val check_clocks_def = Define `
-check_clocks i s1 s2 ⇔
-  s1.clock = i ∧ i ≤ s2.clock`;
+check_clocks f i s1 s2 ⇔
+  s1.clock = i ∧ s2.clock = f i`;
+
+val dec_clock_fn_def = Define `
+dec_clock_fn f (old_start : num) new_start = (\clock. f (clock + (old_start - new_start)))`;
+
+val good_clock_fn_def = Define `
+good_clock_fn (f : num -> num) ⇔
+  (!x y. x ≤ y ⇒ f x ≤ f y) ∧
+  (!x. ?y. x < f y)`;
+
+val good_clock_fn_id = Q.store_thm ("good_clock_fn_id[simp]",
+`good_clock_fn I`,
+ rw [good_clock_fn_def] >>
+ qexists_tac `x + 1` >>
+ simp []);
+
+val dec_clock_fn_id = Q.prove (
+`!f c. dec_clock_fn f c c = f`,
+ rw [dec_clock_fn_def, FUN_EQ_THM]);
+
+val good_clock_fn_dec = Q.prove (
+`!f x y. good_clock_fn f ⇒ good_clock_fn (dec_clock_fn f x y)`,
+ rw [dec_clock_fn_def, good_clock_fn_def] >>
+ pop_assum (qspec_then `x'` mp_tac) >>
+ rw [] >>
+ qexists_tac `y'` >>
+ `y' ≤ y' + (x - y)` by decide_tac >>
+ res_tac >>
+ decide_tac);
 
 val val_rel_def = tDefine "val_rel" `
-(val_rel (i:num) (Number n) (Number n') ⇔ n = n') ∧
-(val_rel i (Block n' vs) (Block n vs') ⇔ n = n' ∧ LIST_REL (val_rel i) vs vs') ∧
-(val_rel i (RefPtr l) (RefPtr l') ⇔ l = l') ∧
-(val_rel i v v' ⇔
+(val_rel (f : num -> num) (i:num) (Number n) (Number n') ⇔ n = n') ∧
+(val_rel f i (Block n' vs) (Block n vs') ⇔ n = n' ∧ LIST_REL (val_rel f i) vs vs') ∧
+(val_rel f i (RefPtr l) (RefPtr l') ⇔ l = l') ∧
+(val_rel f i v v' ⇔
   if is_closure v ∧ is_closure v' then
-    !i'.
-      if i' < i then
-        (!vs vs' s s'.
-          LIST_REL (val_rel i') vs vs' ∧
-          state_rel i' s s' ∧
-          check_clocks i' s s'
-          ⇒ 
-          res_rel (cEvalApp NONE v vs s) (cEvalApp NONE v' vs' s'))
+    !i' vs vs' s s'.
+      if i' < i ∧ check_clocks f i' s s' then
+        LIST_REL (val_rel f i') vs vs' ∧ state_rel f s s' ⇒
+        res_rel (dec_clock_fn f s.clock) (cEvalApp NONE v vs s) (cEvalApp NONE v' vs' s')
       else
-        T
+        T 
   else 
     F) ∧
-(ref_v_rel i (ByteArray ws) (ByteArray ws') ⇔ ws = ws') ∧
-(ref_v_rel i (ValueArray vs) (ValueArray vs') ⇔ LIST_REL (val_rel i) vs vs') ∧
-(ref_v_rel i _ _ ⇔ F) ∧
-(state_rel i s s' ⇔
-  LIST_REL (OPTION_REL (val_rel i)) s.globals s'.globals ∧
-  fmap_rel (ref_v_rel i) s.refs s'.refs ∧
-  fmap_rel (λ(n,e) (n',e'). n = n' ∧ code_rel i [e] [e']) s.code s'.code ∧
+(ref_v_rel f i (ByteArray ws) (ByteArray ws') ⇔ ws = ws') ∧
+(ref_v_rel f i (ValueArray vs) (ValueArray vs') ⇔ LIST_REL (val_rel f i) vs vs') ∧
+(ref_v_rel f i _ _ ⇔ F) ∧
+(state_rel f s s' ⇔
+  LIST_REL (OPTION_REL (val_rel f s.clock)) s.globals s'.globals ∧
+  fmap_rel (ref_v_rel f s.clock) s.refs s'.refs ∧
+  fmap_rel (λ(n,e) (n',e'). n = n' ∧ code_rel f s.clock [e] [e']) s.code s'.code ∧
   s.output = s'.output ∧
   s.restrict_envs = s'.restrict_envs) ∧
-(res_rel (Result vs, s) (Result vs', s') ⇔ 
-  LIST_REL (val_rel s.clock) vs vs' ∧
-  state_rel s.clock s s') ∧
-(res_rel (Exception v, s) (Exception v', s') ⇔ 
-  val_rel s.clock v v' ∧
-  state_rel s.clock s s') ∧
-(res_rel (TimeOut, s) (TimeOut, s') ⇔
-  state_rel s.clock s s') ∧
-(res_rel (Error, s) _ ⇔ T) ∧
-(res_rel _ _ ⇔ F) ∧
-(code_rel i es es' ⇔
+(res_rel (f' : num -> num -> num) (Result vs, s) (Result vs', s') ⇔ 
+  LIST_REL (val_rel (f' s.clock) s.clock) vs vs' ∧
+  state_rel (f' s.clock) s s') ∧
+(res_rel f' (Exception v, s) (Exception v', s') ⇔ 
+  val_rel (f' s.clock) s.clock v v' ∧
+  state_rel (f' s.clock) s s') ∧
+(res_rel f' (TimeOut, s) (TimeOut, s') ⇔
+  state_rel (f' s.clock) s s') ∧
+(res_rel f' (Error, s) _ ⇔ T) ∧
+(res_rel f' _ _ ⇔ F) ∧
+(code_rel f i es es' ⇔
   !env env' s s' i'.
-    i' < i 
-    ⇒
-    LIST_REL (val_rel i') env env' ∧
-    state_rel i' s s' ∧
-    check_clocks i' s s'
-    ⇒
-    res_rel (cEval (es,env,s)) (cEval (es',env',s')))`
+    if i' < i ∧ check_clocks f i' s s' then
+      LIST_REL (val_rel f i') env env' ∧ state_rel f s s' ⇒
+      res_rel (dec_clock_fn f s.clock) (cEval (es,env,s)) (cEval (es',env',s'))
+    else
+      T)`
 (WF_REL_TAC `inv_image ($< LEX $< LEX $<) 
              (\x. case x of 
-                     | INL (i,v,v') => (i:num,0:num,clos_val_size v) 
-                     | INR (INL (i,r,r')) => (i,1,0)
-                     | INR (INR (INL (i,s,s'))) => (i,3,0)
-                     | INR (INR (INR (INL (res,res')))) => ((SND res).clock,4,0)
-                     | INR (INR (INR (INR (i,es,es')))) => (i,2,0))` >>
+                     | INL (f,i,v,v') => (i:num,0:num,clos_val_size v) 
+                     | INR (INL (f,i,r,r')) => (i,1,0)
+                     | INR (INR (INL (f,s,s'))) => (s.clock,3,0)
+                     | INR (INR (INR (INL (f,res,res')))) => ((SND res).clock,4,0)
+                     | INR (INR (INR (INR (f,i,es,es')))) => (i,2,0))` >>
  rw [] >>
  simp [clos_val_size_def] >>
- fs [is_closure_def]
+ fs [is_closure_def, check_clocks_def]
+ >- (Cases_on `cEvalApp NONE (Closure v17 v18 v19 v20 v21) vs s` >>
+     fs [] >>
+     imp_res_tac cEvalApp_clock >>
+     decide_tac)
+ >- (Cases_on `cEvalApp NONE (Recclosure v22 v23 v24 v25 v26) vs s` >>
+     fs [] >>
+     imp_res_tac cEvalApp_clock >>
+     decide_tac)
  >- (Cases_on `cEval (es,env,s)` >>
      fs [check_clocks_def] >>
      rw [] >>
      imp_res_tac cEval_clock >>
      decide_tac)
- >- cheat
- >- cheat >>
- Induct_on `vs` >>
- rw [] >>
- res_tac >>
- simp [clos_val_size_def]);
+ >- (Induct_on `vs` >>
+     rw [] >>
+     res_tac >>
+     simp [clos_val_size_def]));
 
 val val_rel_ind = fetch "-" "val_rel_ind";
 
@@ -169,35 +197,36 @@ val state_rel_rw =
   end;
 
 val exp_rel_def = Define `
-exp_rel es es' ⇔ !i. code_rel i es es'`;
+exp_rel es es' ⇔ !i. ?f. good_clock_fn f ∧ code_rel f i es es'`;
 
 val val_rel_mono = Q.prove (
-`(!i v v'. val_rel i v v' ⇒ ∀i'. i' ≤ i ⇒ val_rel i' v v') ∧
- (!i r r'. ref_v_rel i r r' ⇒ ∀i'. i' ≤ i ⇒ ref_v_rel i' r r') ∧
- (!i s s'. state_rel i s s' ⇒ ∀i'. i' ≤ i ⇒ state_rel i' s s') ∧
- (!res res'. res_rel res res' ⇒ res_rel res res') ∧
- (!i es es'. code_rel i es es' ⇒ ∀i'. i' ≤ i ⇒ code_rel i' es es')`,
+`(!f i v v'. val_rel f i v v' ⇒ ∀i'. i' ≤ i ⇒ val_rel f i' v v') ∧
+ (!f i r r'. ref_v_rel f i r r' ⇒ ∀i'. i' ≤ i ⇒ ref_v_rel f i' r r') ∧
+ (!f s s'. state_rel f s s' ⇒ state_rel f s s') ∧
+ (!f res res'. res_rel f res res' ⇒ res_rel f res res') ∧
+ (!f i es es'. code_rel f i es es' ⇒ ∀i'. i' ≤ i ⇒ code_rel f i' es es')`,
  ho_match_mp_tac val_rel_ind >>
  rw [] >>
  TRY (fs [Once val_rel_def, is_closure_def]  >> NO_TAC)
  >- (fs [val_rel_def, LIST_REL_EL_EQN] >>
      metis_tac [EL_MEM])
- >- (fs [Once val_rel_def] >>
+ >- (fs [val_rel_rw] >>
      Cases_on `v'` >>
      fs [is_closure_def] >>
-     rw [Once val_rel_def, is_closure_def] >>
+     rw [val_rel_rw, is_closure_def] >>
      `i'' < i` by decide_tac >>
      fs [] >>
      metis_tac [])
- >- (fs [Once val_rel_def] >>
+ >- (fs [val_rel_rw] >>
      Cases_on `v'` >>
      fs [is_closure_def] >>
-     rw [Once val_rel_def, is_closure_def] >>
+     rw [val_rel_rw, is_closure_def] >>
      `i'' < i` by decide_tac >>
      fs [] >>
      metis_tac [])
- >- (fs [Once val_rel_def, LIST_REL_EL_EQN] >>
+ >- (fs [val_rel_rw, LIST_REL_EL_EQN] >>
      metis_tac [EL_MEM])
+     (*
  >- (qpat_assum `state_rel i x y` mp_tac >>
      simp [Once val_rel_def] >>
      rw [] >>
@@ -218,7 +247,6 @@ val val_rel_mono = Q.prove (
          pop_assum mp_tac >>
          ASM_REWRITE_TAC [] >>
          simp []))
-         (*
  >- (fs [val_rel_rw] >>
      rw [] >>
      simp [state_rel_rw] >>
@@ -233,7 +261,7 @@ val val_rel_mono = Q.prove (
      fs [LIST_REL_EL_EQN] >>
      metis_tac [EL_MEM])
      *)
- >- (qpat_assum `code_rel i x y` mp_tac >>
+ >- (qpat_assum `code_rel f i x y` mp_tac >>
      simp [Once val_rel_def] >>
      rw [] >>
      simp [Once val_rel_def] >>
@@ -242,19 +270,19 @@ val val_rel_mono = Q.prove (
      metis_tac []));
 
 val val_rel_mono_list = Q.prove (
-`!i i' vs1 vs2.
-  i' ≤ i ∧ LIST_REL (\x y. val_rel i x y) vs1 vs2
+`!f i i' vs1 vs2.
+  i' ≤ i ∧ LIST_REL (\x y. val_rel f i x y) vs1 vs2
   ⇒
-  LIST_REL (\x y. val_rel i' x y) vs1 vs2`,
+  LIST_REL (\x y. val_rel f i' x y) vs1 vs2`,
  rw [LIST_REL_EL_EQN] >>
  metis_tac [val_rel_mono]);
 
 val exp_rel_empty = Q.prove (
 `exp_rel [] []`,
  rw [exp_rel_def, cEval_def, val_rel_rw] >>
+ qexists_tac `I` >>
  rw [code_rel_rw, val_rel_rw, cEval_def] >>
- `i' - s.clock ≤ i'` by decide_tac >>
- metis_tac [val_rel_mono, check_clocks_def]);
+ metis_tac [dec_clock_fn_id, val_rel_mono, check_clocks_def]);
 
  (*
 val exp_rel_cons = Q.prove (
@@ -263,11 +291,15 @@ val exp_rel_cons = Q.prove (
   exp_rel es es'
   ⇒
   exp_rel (e::es) (e'::es')`,
- rw [exp_rel_def, code_rel_rw] >>
+
+ rw [exp_rel_def, code_rel_rw, SKOLEM_THM] >>
  ONCE_REWRITE_TAC [cEval_CONS] >>
+ ntac 2 (last_x_assum (qspec_then `i` strip_assume_tac)) >>
+ qexists_tac 
  Cases_on `cEval ([e],env,s)` >>
  Cases_on `q` >>
- fs [] >>
+
+
  `res_rel (cEval ([e],env,s)) (cEval ([e'],env',s'))` by metis_tac [] >>
  fs [] >>
  rw [] >>
@@ -279,14 +311,14 @@ val exp_rel_cons = Q.prove (
  fs [val_rel_rw] >>
  imp_res_tac cEval_clock >>
  `r.clock ≤ i' ∧ r.clock < i` by (fs [check_clocks_def] >> decide_tac) >>
- `LIST_REL (λa' a. val_rel r.clock a' a) env env'` by metis_tac [val_rel_mono_list] >>
+ `LIST_REL (λa' a. val_rel f r.clock a' a) env env'` by metis_tac [val_rel_mono_list] >>
 
- `check_clocks r.clock r r'` by cheat >>
- `res_rel (cEval (es,env,r)) (cEval (es',env',r'))` by metis_tac [val_rel_mono, val_rel_mono_list] >>
+ `check_clocks f r.clock r r'` by (fs [state_rel_rw, check_clocks_def])
+ `res_rel f (cEval (es,env,r)) (cEval (es',env',r'))` by metis_tac [val_rel_mono, val_rel_mono_list] >>
  ect >>
  fs [] >>
  rw [] >>
- fs [val_rel_rw, LIST_REL_EL_EQN] >>
+ simp [val_rel_rw, LIST_REL_EL_EQN] >>
  imp_res_tac cEval_length_imp >>
  Cases_on `a` >>
  fs [] >>
